Logic/FirstOrder/Basic/Language.lean
@@ -8,14 +8,14 @@ open Primrec
 namespace FirstOrder
 
 structure Language where
-  func : Nat → Type u
-  rel  : Nat → Type u
+  Func : Nat → Type u
+  Rel  : Nat → Type u
 
 namespace Language
 
 protected def empty : Language.{u} where
-  func := fun _ => PEmpty
-  rel  := fun _ => PEmpty
+  Func := fun _ => PEmpty
+  Rel  := fun _ => PEmpty
 
 instance : Inhabited Language := ⟨Language.empty⟩
 
@@ -28,8 +28,8 @@ inductive GraphRel : ℕ → Type
   | le : GraphRel 2
 
 def graph : Language where
-  func := GraphFunc
-  rel := GraphRel
+  Func := GraphFunc
+  Rel := GraphRel
 
 inductive BinaryRel : ℕ → Type
   | isone : BinaryRel 1
@@ -37,28 +37,28 @@ inductive BinaryRel : ℕ → Type
   | le : BinaryRel 2
 
 def binary : Language where
-  func := fun _ => Empty
-  rel := BinaryRel
+  Func := fun _ => Empty
+  Rel := BinaryRel
 
 inductive EqRel : ℕ → Type
   | equal : EqRel 2
 
 @[reducible]
 def equal : Language where
-  func := fun _ => Empty
-  rel := EqRel
+  Func := fun _ => Empty
+  Rel := EqRel
 
-instance (k) : ToString (equal.func k) := ⟨fun _ => ""⟩
+instance (k) : ToString (equal.Func k) := ⟨fun _ => ""⟩
 
-instance (k) : ToString (equal.rel k) := ⟨fun _ => "\\mathrm{Eq}"⟩
+instance (k) : ToString (equal.Rel k) := ⟨fun _ => "\\mathrm{Eq}"⟩
 
-instance (k) : DecidableEq (equal.func k) := fun a b => by rcases a
+instance (k) : DecidableEq (equal.Func k) := fun a b => by rcases a
 
-instance (k) : DecidableEq (equal.rel k) := fun a b => by rcases a; rcases b; exact isTrue (by simp)
+instance (k) : DecidableEq (equal.Rel k) := fun a b => by rcases a; rcases b; exact isTrue (by simp)
 
-instance (k) : Encodable (equal.func k) := IsEmpty.toEncodable
+instance (k) : Encodable (equal.Func k) := IsEmpty.toEncodable
 
-instance (k) : Encodable (equal.rel k) where
+instance (k) : Encodable (equal.Rel k) where
   encode := fun _ => 0
   decode := fun _ =>
     match k with
@@ -82,12 +82,12 @@ end ORing
 
 @[reducible]
 def oRing : Language where
-  func := ORing.Func
-  rel := ORing.Rel
+  Func := ORing.Func
+  Rel := ORing.Rel
 
 namespace ORing
 
-instance (k) : ToString (oRing.func k) :=
+instance (k) : ToString (oRing.Func k) :=
 ⟨ fun s =>
   match s with
   | Func.zero => "0"
@@ -95,19 +95,19 @@ instance (k) : ToString (oRing.func k) :=
   | Func.add  => "(+)"
   | Func.mul  => "(\\cdot)"⟩
 
-instance (k) : ToString (oRing.rel k) :=
+instance (k) : ToString (oRing.Rel k) :=
 ⟨ fun s =>
   match s with
   | Rel.eq => "\\mathrm{Eq}"
   | Rel.lt    => "\\mathrm{LT}"⟩
 
-instance (k) : DecidableEq (oRing.func k) := fun a b =>
+instance (k) : DecidableEq (oRing.Func k) := fun a b =>
   by rcases a <;> rcases b <;> simp <;> try {exact instDecidableTrue} <;> try {exact instDecidableFalse}
 
-instance (k) : DecidableEq (oRing.rel k) := fun a b =>
+instance (k) : DecidableEq (oRing.Rel k) := fun a b =>
   by rcases a <;> rcases b <;> simp <;> try {exact instDecidableTrue} <;> try {exact instDecidableFalse}
 
-instance (k) : Encodable (oRing.func k) where
+instance (k) : Encodable (oRing.Func k) where
   encode := fun x =>
     match x with
     | Func.zero => 0
@@ -123,9 +123,9 @@ instance (k) : Encodable (oRing.func k) where
     | _, _ => none
   encodek := fun x => by rcases x <;> simp
 
-instance Func1IsEmpty : IsEmpty (oRing.func 1) := ⟨by rintro ⟨⟩⟩
+instance Func1IsEmpty : IsEmpty (oRing.Func 1) := ⟨by rintro ⟨⟩⟩
 
-instance FuncGe3IsEmpty : ∀ k ≥ 3, IsEmpty (oRing.func k)
+instance FuncGe3IsEmpty : ∀ k ≥ 3, IsEmpty (oRing.Func k)
   | 0       => by simp
   | 1       => by simp
   | 2       => by simp
@@ -143,7 +143,7 @@ private lemma Func_encodeDecode_primrec : Primrec₂ (fun k e =>
       <| Primrec.ite (PrimrecPred.and (Primrec.eq.comp fst (const _)) (Primrec.eq.comp snd (const _))) (const _)
       <| const _
 
-instance (k) : Primcodable (oRing.func k) where
+instance (k) : Primcodable (oRing.Func k) where
   prim := nat_iff.mp <| (Primrec.encode.comp (Func_encodeDecode_primrec.comp (Primrec.const k) Primrec.id)).of_eq (fun e => by
     simp[Encodable.decode]
     rcases k with (_ | k)
@@ -152,7 +152,7 @@ instance (k) : Primcodable (oRing.func k) where
       · rcases k with (_ | k) <;> simp
         · rcases e with (_ | e) <;> simp; rcases e with (_ | e) <;> simp)
 
-instance : UniformlyPrimcodable oRing.func := UniformlyPrimcodable.ofEncodeDecode
+instance : UniformlyPrimcodable oRing.Func := UniformlyPrimcodable.ofEncodeDecode
   (Func_encodeDecode_primrec.of_eq $ fun k e => by
     simp[Encodable.encodeDecode, Encodable.decode]
     rcases k with (_ | k)
@@ -161,7 +161,7 @@ instance : UniformlyPrimcodable oRing.func := UniformlyPrimcodable.ofEncodeDecod
       · rcases k with (_ | k) <;> simp
         · rcases e with (_ | e) <;> simp; rcases e with (_ | e) <;> simp)
 
-instance (k) : Encodable (oRing.rel k) where
+instance (k) : Encodable (oRing.Rel k) where
   encode := fun x =>
     match x with
     | Rel.eq => 0
@@ -181,7 +181,7 @@ private lemma Rel_encodeDecode_primrec : Primrec₂ (fun k e =>
       <| Primrec.ite (PrimrecPred.and (Primrec.eq.comp fst (const _)) (Primrec.eq.comp snd (const _))) (const _)
       <| const _
 
-instance (k) : Primcodable (oRing.rel k) where
+instance (k) : Primcodable (oRing.Rel k) where
   prim := nat_iff.mp <| (Primrec.encode.comp (Rel_encodeDecode_primrec.comp (Primrec.const k) Primrec.id)).of_eq (fun e => by
     simp[Encodable.decode]
     rcases k with (_ | k) <;> simp
@@ -190,7 +190,7 @@ instance (k) : Primcodable (oRing.rel k) where
     rcases e with (_ | e) <;> simp
     rcases e with (_ | e) <;> simp)
 
-instance : UniformlyPrimcodable oRing.rel := UniformlyPrimcodable.ofEncodeDecode
+instance : UniformlyPrimcodable oRing.Rel := UniformlyPrimcodable.ofEncodeDecode
   (Rel_encodeDecode_primrec.of_eq $ fun k e => by
     simp[Encodable.encodeDecode, Encodable.decode]
     rcases k with (_ | k) <;> simp
@@ -202,55 +202,55 @@ instance : UniformlyPrimcodable oRing.rel := UniformlyPrimcodable.ofEncodeDecode
 end ORing
 
 def relational (α : ℕ → Type u) : Language where
-  func := fun _ => PEmpty
-  rel := α
+  Func := fun _ => PEmpty
+  Rel := α
 
 section relational
 variable {α : ℕ → Type u} [e : ∀ n, Encodable (α n)] [d : ∀ n, DecidableEq (α n)] [s : ∀ n, ToString (α n)]
 
-instance (k) : Encodable ((relational α).func k) := IsEmpty.toEncodable (α := PEmpty)
+instance (k) : Encodable ((relational α).Func k) := IsEmpty.toEncodable (α := PEmpty)
 
-instance (k) : Encodable ((relational α).rel k) := e k
+instance (k) : Encodable ((relational α).Rel k) := e k
 
-instance (k) : DecidableEq ((relational α).func k) := fun a => by cases a
+instance (k) : DecidableEq ((relational α).Func k) := fun a => by cases a
 
-instance (k) : DecidableEq ((relational α).rel k) := d k
+instance (k) : DecidableEq ((relational α).Rel k) := d k
 
-instance : ToString ((relational α).rel k) :=
+instance : ToString ((relational α).Rel k) :=
   ⟨fun a => "R^{" ++ toString k ++ "}_{" ++ toString (α := α k) a ++ "}"⟩
 
-def toRelational (a : α k) : (relational α).rel k := a
+def toRelational (a : α k) : (relational α).Rel k := a
 
-instance : ToString ((relational α).func k) := ⟨fun a => by cases a⟩
+instance : ToString ((relational α).Func k) := ⟨fun a => by cases a⟩
 
 end relational
 
 protected class Eq (L : Language.{u}) where
-  eq : L.rel 2
+  eq : L.Rel 2
 
 protected class LT (L : Language.{u}) where
-  lt : L.rel 2
+  lt : L.Rel 2
 
 protected class Zero (L : Language.{u}) where
-  zero : L.func 0
+  zero : L.Func 0
 
 protected class One (L : Language.{u}) where
-  one : L.func 0
+  one : L.Func 0
 
 protected class Add (L : Language.{u}) where
-  add : L.func 2
+  add : L.Func 2
 
 protected class Mul (L : Language.{u}) where
-  mul : L.func 2
+  mul : L.Func 2
 
 protected class Pow (L : Language.{u}) where
-  pow : L.func 2
+  pow : L.Func 2
 
 protected class Exp (L : Language.{u}) where
-  exp : L.func 1
+  exp : L.Func 1
 
 class Pairing (L : Language.{u}) where
-  pair : L.func 2
+  pair : L.Func 2
 
 attribute [match_pattern] Zero.zero One.one Add.add Mul.mul Eq.eq LT.lt
 
@@ -269,7 +269,7 @@ namespace ORing
 
 open Qq Lean Elab Meta Tactic
 
-def denoteFunc : (k : ℕ) → Q(oRing.func $k) → MetaM (oRing.func k)
+def denoteFunc : (k : ℕ) → Q(oRing.Func $k) → MetaM (oRing.Func k)
   | 0, e =>
     match e with
     | ~q(Zero.zero) => return Language.Zero.zero
@@ -280,28 +280,28 @@ def denoteFunc : (k : ℕ) → Q(oRing.func $k) → MetaM (oRing.func k)
     | ~q(Language.Mul.mul) => return Language.Mul.mul
   | _, e => throwError m!"error in DenotationORing : {e}"
 
-def denoteRel : (k : ℕ) → Q(oRing.rel $k) → MetaM (oRing.rel k)
+def denoteRel : (k : ℕ) → Q(oRing.Rel $k) → MetaM (oRing.Rel k)
   | 2, e =>
     match e with
     | ~q(Language.Eq.eq) => return Language.Eq.eq
     | ~q(Language.LT.lt) => return Language.LT.lt
   | _, e => throwError m!"error in DenotationORing : {e}"
 
-instance (k : ℕ) : Denotation q(oRing.func $k) (oRing.func k) where
+instance (k : ℕ) : Denotation q(oRing.Func $k) (oRing.Func k) where
    denote := denoteFunc k
    toExpr := fun f =>
      ( match f with
        | Func.zero => q(Language.Zero.zero)
        | Func.one  => q(Language.One.one)
        | Func.add  => q(Language.Add.add)
-       | Func.mul  => q(Language.Mul.mul) : Q(oRing.func $k))
+       | Func.mul  => q(Language.Mul.mul) : Q(oRing.Func $k))
 
-instance (k : ℕ) : Denotation q(oRing.rel $k) (oRing.rel k) where
+instance (k : ℕ) : Denotation q(oRing.Rel $k) (oRing.Rel k) where
    denote := denoteRel k
    toExpr := fun f =>
      ( match f with
        | Rel.eq => q(Language.Eq.eq)
-       | Rel.lt => q(Language.LT.lt) : Q(oRing.rel $k))
+       | Rel.lt => q(Language.LT.lt) : Q(oRing.Rel $k))
 
 end ORing
 -/
@@ -309,15 +309,15 @@ end ORing
 def ofFunc (F : ℕ → Type v) : Language := ⟨F, fun _ => PEmpty⟩
 
 def add (L₁ : Language.{u₁}) (L₂ : Language.{u₂}) : Language :=
-  ⟨fun k => L₁.func k ⊕ L₂.func k, fun k => L₁.rel k ⊕ L₂.rel k⟩
+  ⟨fun k => L₁.Func k ⊕ L₂.Func k, fun k => L₁.Rel k ⊕ L₂.Rel k⟩
 
 instance : _root_.Add Language := ⟨add⟩
 
-def sigma (L : ι → Language) : Language := ⟨fun k => Σ i, (L i).func k, fun k => Σ i, (L i).rel k⟩
+def sigma (L : ι → Language) : Language := ⟨fun k => Σ i, (L i).Func k, fun k => Σ i, (L i).Rel k⟩
 
 @[ext] structure Hom (L₁ L₂ : Language) where
-  func : {k : ℕ} → L₁.func k → L₂.func k
-  rel : {k : ℕ} → L₁.rel k → L₂.rel k
+  func : {k : ℕ} → L₁.Func k → L₂.Func k
+  rel : {k : ℕ} → L₁.Rel k → L₂.Rel k
 
 scoped[LO.FirstOrder] infix:25 " →ᵥ " => LO.FirstOrder.Language.Hom
 
@@ -338,23 +338,23 @@ def add₁ (L₁ : Language.{u₁}) (L₂ : Language.{u₂}) : L₁ →ᵥ L₁.
 
 def add₂ (L₁ : Language.{u₁}) (L₂ : Language.{u₂}) : L₂ →ᵥ L₁.add L₂ := ⟨Sum.inr, Sum.inr⟩
 
-@[simp] lemma func_add₁ (L₁ : Language.{u₁}) (L₂ : Language.{u₂}) (f : L₁.func k) :
+@[simp] lemma func_add₁ (L₁ : Language.{u₁}) (L₂ : Language.{u₂}) (f : L₁.Func k) :
     (add₁ L₁ L₂).func f = Sum.inl f := rfl
 
-@[simp] lemma rel_add₁ (L₁ : Language.{u₁}) (L₂ : Language.{u₂}) (r : L₁.rel k) :
+@[simp] lemma rel_add₁ (L₁ : Language.{u₁}) (L₂ : Language.{u₂}) (r : L₁.Rel k) :
     (add₁ L₁ L₂).rel r = Sum.inl r := rfl
 
-@[simp] lemma func_add₂ (L₁ : Language.{u₁}) (L₂ : Language.{u₂}) (f : L₂.func k) :
+@[simp] lemma func_add₂ (L₁ : Language.{u₁}) (L₂ : Language.{u₂}) (f : L₂.Func k) :
     (add₂ L₁ L₂).func f = Sum.inr f := rfl
 
-@[simp] lemma rel_add₂ (L₁ : Language.{u₁}) (L₂ : Language.{u₂}) (r : L₂.rel k) :
+@[simp] lemma rel_add₂ (L₁ : Language.{u₁}) (L₂ : Language.{u₂}) (r : L₂.Rel k) :
     (add₂ L₁ L₂).rel r = Sum.inr r := rfl
 
 def sigma (L : ι → Language) (i : ι) : L i →ᵥ Language.sigma L := ⟨fun f => ⟨i, f⟩, fun r => ⟨i, r⟩⟩
 
-@[simp] lemma func_sigma (L : ι → Language) (i : ι) (f : (L i).func k) : (sigma L i).func f = ⟨i, f⟩ := rfl
+@[simp] lemma func_sigma (L : ι → Language) (i : ι) (f : (L i).Func k) : (sigma L i).func f = ⟨i, f⟩ := rfl
 
-@[simp] lemma rel_sigma (L : ι → Language) (i : ι) (r : (L i).rel k) : (sigma L i).rel r = ⟨i, r⟩ := rfl
+@[simp] lemma rel_sigma (L : ι → Language) (i : ι) (r : (L i).Rel k) : (sigma L i).rel r = ⟨i, r⟩ := rfl
 
 end Hom
 
