Logic/FirstOrder/Basic/Soundness.lean
@@ -7,7 +7,7 @@ namespace FirstOrder
 
 section soundness
 
-variable {L : Language.{u}} [∀ k, DecidableEq (L.func k)] [∀ k, DecidableEq (L.rel k)]
+variable {L : Language.{u}} [∀ k, DecidableEq (L.Func k)] [∀ k, DecidableEq (L.Rel k)]
 
 variable {P : SyntacticFormula L → Prop}
 
