Logic/FirstOrder/Computability/Calculus.lean
@@ -7,16 +7,16 @@ namespace LO
 namespace FirstOrder
 
 open Encodable
-variable {L : Language.{u}} [∀ k, DecidableEq (L.func k)] [∀ k, DecidableEq (L.rel k)]
-variable [(k : ℕ) → Primcodable (L.func k)] [(k : ℕ) → Primcodable (L.rel k)]
-  [UniformlyPrimcodable L.func] [UniformlyPrimcodable L.rel] [Primcodable μ]
+variable {L : Language.{u}} [∀ k, DecidableEq (L.Func k)] [∀ k, DecidableEq (L.Rel k)]
+variable [(k : ℕ) → Primcodable (L.Func k)] [(k : ℕ) → Primcodable (L.Rel k)]
+  [UniformlyPrimcodable L.Func] [UniformlyPrimcodable L.Rel] [Primcodable μ]
 
 namespace Derivation
 
 open DerivationCR
 
 inductive Code (L : Language.{u})
-  | axL : {k : ℕ} → (r : L.rel k) → (v : Fin k → SyntacticTerm L) → Code L
+  | axL : {k : ℕ} → (r : L.Rel k) → (v : Fin k → SyntacticTerm L) → Code L
   | verum : Code L
   | and : SyntacticFormula L → SyntacticFormula L → Code L
   | or : SyntacticFormula L → SyntacticFormula L → Code L
@@ -26,7 +26,7 @@ inductive Code (L : Language.{u})
 
 def Code.equiv (L : Language.{u}) :
     Code L ≃
-    ((k : ℕ) × (L.rel k) × (Fin k → SyntacticTerm L)) ⊕
+    ((k : ℕ) × (L.Rel k) × (Fin k → SyntacticTerm L)) ⊕
     Unit ⊕
     (SyntacticFormula L × SyntacticFormula L) ⊕
     (SyntacticFormula L × SyntacticFormula L) ⊕
