Logic/FirstOrder/Order/Le.lean
@@ -7,7 +7,7 @@ namespace LO
 namespace FirstOrder
 
 variable {L : Language.{u}} [Subformula.Operator.Eq L] [Subformula.Operator.LT L]
-  [∀ k, DecidableEq (L.func k)] [∀ k, DecidableEq (L.rel k)]
+  [∀ k, DecidableEq (L.Func k)] [∀ k, DecidableEq (L.Rel k)]
 
 open Subformula
 
